Look at assign_thm in bvp_to_wordProof
Have not proved any cases yet.

It seems like there might be problems in the semantics regarding
globals.

For the case I looked at that looks provable, I don't know enough about
the data refinement to know what the appropriate state_rel set_var
theorem should be.

compiler/backend/bvp_to_wordScript.sml
@@ -25,6 +25,7 @@ val assign_def = Define `
         if i < 0
         then (Assign (adjust_var dest) (Const (0w - n2w (Num (4 * (0 - i))))),l)
         else (Assign (adjust_var dest) (Const (n2w (Num (4 * i)))),l)
+    | GlobalsPtr => (Assign (adjust_var dest) (Lookup Globals),l)
     | _ => (Skip:'a wordLang$prog,l)`;
 
 val comp_def = Define `
